Add more to equivilence

examples/computability/turingMachines/.#turing_machineScript.sml
@@ -1,0 +1,1 @@
+elliotcatt@Aisha.local.47401
